Engine: add begin and jumps in tree_rep

Engine/TreeRep.v
@@ -12,53 +12,63 @@ From Warblre Require Import Base.
 (* A predicate showing that a tree is represented at a given point in the code *)
 
 
-Inductive tree_rep: tree -> code -> label -> input -> LoopBool -> Prop :=
+Inductive tree_rep: tree -> code -> label -> input -> LoopBool -> nat -> Prop :=
 | tr_match:
   forall code pc inp b
     (ACCEPT: get_pc code pc = Some Accept),
-    tree_rep Match code pc inp b
+    tree_rep Match code pc inp b 0
+| tr_jmp:
+  forall code pc nextpc inp b t n
+    (JMP: get_pc code pc = Some (Jmp nextpc))
+    (TR: tree_rep t code nextpc inp b n),
+    tree_rep t code pc inp b (S n)
+| tr_begin:
+  forall code pc inp b t n
+    (BEGIN: get_pc code pc = Some BeginLoop)
+    (TR: tree_rep t code (S pc) inp CannotExit n),
+    tree_rep t code pc inp b n
 | tr_choice:
-  forall code pc pc1 pc2 inp b t1 t2
+  forall code pc pc1 pc2 inp b t1 t2 n1 n2
     (FORK: get_pc code pc = Some (Fork pc1 pc2))
-    (TR1: tree_rep t1 code pc1 inp b)
-    (TR2: tree_rep t2 code pc2 inp b),
-    tree_rep (Choice t1 t2) code pc inp b
+    (TR1: tree_rep t1 code pc1 inp b n1)
+    (TR2: tree_rep t2 code pc2 inp b n2),
+    tree_rep (Choice t1 t2) code pc inp b (n1 + n2)
 | tr_read:
-  forall code pc inp nextinp b cd c t
+  forall code pc inp nextinp b cd c t n
     (CONSUME: get_pc code pc = Some (Consume cd))
     (READ: read_char cd inp forward = Some (c, nextinp))
-    (TR: tree_rep t code (S pc) nextinp CanExit),
-    tree_rep (Read c t) code pc inp b
+    (TR: tree_rep t code (S pc) nextinp CanExit n),
+    tree_rep (Read c t) code pc inp b n
 | tr_progress:
-  forall code pc nextpc inp t
+  forall code pc nextpc inp t n
     (ENDLOOP: get_pc code pc = Some (EndLoop nextpc))
-    (TR: tree_rep t code nextpc inp CanExit),
-    tree_rep (Progress t) code pc inp CanExit
+    (TR: tree_rep t code nextpc inp CanExit n),
+    tree_rep (Progress t) code pc inp CanExit n
 | tr_open:
-  forall code pc gid inp b t
+  forall code pc gid inp b t n
     (OPEN: get_pc code pc = Some (SetRegOpen gid))
-    (TR: tree_rep t code (S pc) inp b),
-    tree_rep (GroupAction (Open gid) t) code pc inp b
+    (TR: tree_rep t code (S pc) inp b n),
+    tree_rep (GroupAction (Open gid) t) code pc inp b n
 | tr_close:
-  forall code pc gid inp b t
+  forall code pc gid inp b t n
     (CLOSE: get_pc code pc = Some (SetRegClose gid))
-    (TR: tree_rep t code (S pc) inp b),
-    tree_rep (GroupAction (Close gid) t) code pc inp b
+    (TR: tree_rep t code (S pc) inp b n),
+    tree_rep (GroupAction (Close gid) t) code pc inp b n
 | tr_reset:
-  forall code pc gidl inp b t
+  forall code pc gidl inp b t n
     (RESET: get_pc code pc = Some (ResetRegs gidl))
-    (TR: tree_rep t code (S pc) inp b),
-    tree_rep (GroupAction (Reset gidl) t) code pc inp b
+    (TR: tree_rep t code (S pc) inp b n),
+    tree_rep (GroupAction (Reset gidl) t) code pc inp b n
 | tr_readfail:
   forall code pc inp b cd
     (CONSUME: get_pc code pc = Some (Consume cd))
     (READ: read_char cd inp forward = None),
-    tree_rep Mismatch code pc inp b
+    tree_rep Mismatch code pc inp b 0
 | tr_progressfail:
   forall code pc nextpc inp
     (ENDLOOP: get_pc code pc = Some (EndLoop nextpc)),
-    tree_rep Mismatch code pc inp CannotExit.
-  
+    tree_rep Mismatch code pc inp CannotExit 0.
+
 
 Ltac same_instr :=
   match goal with
@@ -67,23 +77,39 @@ Ltac same_instr :=
 
 (* Determinism of the tree representation *)
 Lemma tree_rep_determ:
-  forall code pc inp b t1 t2,
-    tree_rep t1 code pc inp b ->
-    tree_rep t2 code pc inp b ->
-    t1 = t2.
+  forall code pc inp b t1 t2 n1 n2,
+    tree_rep t1 code pc inp b n1 ->
+    tree_rep t2 code pc inp b n2 ->
+    t1 = t2 /\ n1 = n2.
 Proof.
-  intros code pc inp b t1 t2 H H0.
-  generalize dependent t2. induction H; intros.
+  intros code pc inp b t1 t2 n1 n2 H H0.
+  generalize dependent t2. generalize dependent n2.
+  induction H; intros.
+  - inversion H0; subst; auto; same_instr.
+  - inversion H0; subst; auto; same_instr.
+    specialize (IHtree_rep _ _ TR) as [EQT EQN].
+    subst. split; auto.
   - inversion H0; subst; auto; same_instr.
   - inversion H1; subst; auto; same_instr.
-    subst. f_equal; auto.
+    specialize (IHtree_rep1 _ _ TR1) as [EQT1 EQN1].
+    specialize (IHtree_rep2 _ _ TR2) as [EQT2 EQN2].
+    subst. split; auto.
+  - inversion H0; subst; auto; same_instr;
+      rewrite READ0 in READ; inversion READ; subst.
+    specialize (IHtree_rep _ _ TR) as [EQT EQN].
+    subst. split; auto.
   - inversion H0; subst; auto; same_instr.
-    + rewrite READ0 in READ. inversion READ. subst. f_equal; auto.
-    + rewrite READ0 in READ. inversion READ.
-  - inversion H0; subst; auto; same_instr. f_equal; auto.
-  - inversion H0; subst; auto; same_instr. f_equal; auto.
-  - inversion H0; subst; auto; same_instr. f_equal; auto.
-  - inversion H0; subst; auto; same_instr. f_equal; auto.
+    specialize (IHtree_rep _ _ TR) as [EQT EQN].
+    subst. split; auto.
+  - inversion H0; subst; auto; same_instr.
+    specialize (IHtree_rep _ _ TR) as [EQT EQN].
+    subst. split; auto.
+  - inversion H0; subst; auto; same_instr.
+    specialize (IHtree_rep _ _ TR) as [EQT EQN].
+    subst. split; auto.
+  - inversion H0; subst; auto; same_instr.
+    specialize (IHtree_rep _ _ TR) as [EQT EQN].
+    subst. split; auto.
   - inversion H0; subst; auto; same_instr.
     rewrite READ0 in READ. inversion READ.
   - inversion H0; subst; auto; same_instr.
